ROOT
@@ -7,7 +7,6 @@ theories
   "GExp"
   "GExp_Lexorder"
   "efsm-ltl/EFSM_LTL"
-  "efsm-ltl/LTL_Exp"
   "Contexts"
   "AExp"
   "AExp_Lexorder"
